Finding the marginal Pdf of X and Y
\begin{align}
f_{X}(x)&=\int_{0}^{1} f_{X,Y}(x,y)\;dy\\
&=\int_{0}^{1} (x+y)\;dy\\
f_{Y}(y)&=\int_{0}^{1} f_{X,Y}(x,y)\;dx\\
&=\int_{0}^{1} (x+y)\;dx\\
\end{align}
We get
\begin{align}
f_{X}(x)=  \begin{cases}
    x+1/2 & 0\leq x \leq 1 \\
    0 & otherwise
\end{cases}    
\end{align}
\begin{align}
f_{Y}(y)=  \begin{cases}
    y+1/2 & 0\leq y \leq 1 \\
    0 & otherwise
\end{cases}
\end{align}
Finding the marginal Cdf of Y
\begin{align}
F_{Y}(y)&=\int _{0 }^{y}f_{Y}(t)\,dt \\ 
&=\int _{0 }^{y}\brak{t+\frac{1}{2}}\,dt \\ 
\end{align}
We get 
\begin{align}
 F_{Y}(y)=  \begin{cases}
    0  & y\leq 0 \\  
    \frac{y^2+y}{2} & 0\leq y \leq 1 \\
    1 & otherwise
\end{cases}   
\end{align}
\begin{align}
\pr{X+Y\leq 1}&=\pr{Y\leq 1-X} \\
&=\int_{0}^{1} \pr{Y \leq 1-x|X=x}f_X(x)\;dx
\\
&=\int_{0}^{1} F_Y(1-x)\times f_X(x)\;dx
\\
&=\int_{0}^{1}F_Y(x)\times f_X(1-x)\;dx 
\\
&=\int_{0}^{1} \brak{\frac{x+x^2}{2} }\brak{\frac{3-2x}{2}}\;dx
\\
&=\int_{0}^{1} \brak{\frac{3x+x^2-2x^3}{4} }\;dx
\\
&= \frac{1}{4}\sbrak{{\frac{3x^2}{2}+\frac{x^3}{3}-\frac{2x^4}{4}}}_{0}^{1}
\\
&=\frac{1}{3}
\end{align}