If $X$ is a random variable, the cumulative distribution functions of U and 2V can be written in terms of $X$ as
\begin{align} \label{equation-1}
    F(x)=\pr{X \leq x} 
\end{align}
\begin{align}
    G(x)=\pr{2X \leq x}
\end{align}
Or,
\begin{align} \label{equation-2}
     G(x)=\pr{X \leq x/2}
\end{align}
Using \ref{equation-1} in \ref{equation-2}, we can see that
\begin{align} \label{equation-3}
    G(x)=F(x/2)
\end{align}
So,
\begin{align}
    F(x)-G(x)=F(x)-F(x/2)
\end{align}
As F is Cumulative Distribution Function, it is non-decreasing.\\
That means for $x \geq y$, $F(x) \geq F(y)$.\\ \\
Using this, we can form the following table:
\begin{table}[h!]
    \centering
    \begin{tabular}{|c|c|c|}
        \hline
        Case & $F(x)-F(x/2)$ & $(F(x)-F(x/2))x$ \\
        \hline
        $x \geq 0$ & $\geq 0$ & $\geq 0$ \\
        \hline
        $x \leq 0$ & $\leq 0$ & $\geq 0$ \\
        \hline
    \end{tabular}
    \caption{}
    \label{table-1}
\end{table}\\
From the table we can see that for any value of $x$,
\begin{align}
    (F(x)-F(x/2))x \geq 0
\end{align}
Or, using \ref{equation-3},
\begin{align}
    (F(x)-G(x))x \geq x
\end{align}