Before we start the proof we need to know 3 properties of expectation
\begin{equation}
E[f\brak{x}+g\brak{x}] = E[f\brak{x}]+E[g\brak{x}]
\end{equation}
If $k$ is a constant value then 
\begin{align}
E[k\cdot g\brak{x}] &= k\cdot E[g\brak{x}]\\
E[k]&=k
\end{align}
Now variance of random $X$ is given by 
\begin{align}
\nonumber \nonumber Var\brak{X} &= E[\brak{X-\mu}^2] \quad \text{where} \: \mu =E[X]\\
\nonumber \\
\nonumber Var\brak{X}&= E[X^2-2\mu\cdot X + \mu^2]\\
\nonumber\\
\nonumber &= E[X^2]-E[2\mu\cdot X] + E[\mu^2] \:\: \text{from } \brak{1}\\
\nonumber\\
\nonumber &=E[X^2]-2\mu\cdot E[X] + \mu^2 \:\: \text{from} \brak{2} \text{and} \brak{3}\\
\nonumber \\
\nonumber &=E[X^2]-2\mu^2+\mu^2 \quad \brak{\because E[X]=\mu}\\
\nonumber \\
\nonumber &= E[X^2]-\mu^2\\
\nonumber \\
\nonumber &= E[X^2]-E^2[X] \quad \brak{\because \: \mu = E[X]}
\end{align}
