pdf of $X$ is :
\begin{align}
    f_X(x)&=\int_{-\infty}^{\infty}f(x,y)dy\\
    &=\int_{-\sqrt{1-x^2}}^{\sqrt{1-x^2}}\frac{1}{\pi}dy\\
    &=\frac{2\sqrt{1-x^2}}{\pi}
\end{align}
pdf of $Y$ is :
\begin{align}
    f_Y(y)&=\int_{-\infty}^{\infty}f(x,y)dx\\
    &=\int_{-\sqrt{1-y^2}}^{\sqrt{1-y^2}}\frac{1}{\pi}dx\\
    &=\frac{2\sqrt{1-y^2}}{\pi}
\end{align}
cdf of $Y$ is:
\begin{align}
    F_Y(y)&=\int_{-\infty}^{y}f_Y(y)dy\\
    &=\int_{-1}^{y}\frac{2\sqrt{1-y^2}}{\pi}dy\\
    &=\frac{2}{\pi}\sbrak{\dfrac{\sin^{-1}{y} + y\sqrt{1-y^2}}{2} + \frac{\pi}{4}}
\end{align}
The value of $\pr{-X<Y<X}$ is:
\begin{align}
\pr{-X<Y<X} &=F_Y(X)-F_Y(-X)\\
 &=\frac{2}{\pi}\brak{\sin^{-1}{X} + X\sqrt{1-X^2}}
\end{align}
Integrating our probability over all of $X$ we get the value of $ E[\pr{-x<Y<x}]$ as 
\begin{align}
&=\int_{-\infty}^{\infty}f_X(x)\pr{-x<Y<x}dx\\
    &=\brak{\frac{2}{\pi}}^2\int_0^1\sqrt{1-x^2}\brak{\sin^{-1}{x} + x\sqrt{1-x^2}}dx
\end{align}
Substituting
\begin{align} 
u &= \sin^{-1}{x} + x\sqrt{1-x^2}\\
\frac{du}{dx} &= 2\sqrt{1-x^2}\\
&=\brak{\frac{2}{\pi}}^2\int_0^{\frac{\pi}{2}}\frac{u}{2}du\\
&=\brak{\frac{2}{\pi}}^2\brak{\frac{u^2}{4}} \bigg |_0^{\frac{\pi}{2}}\\
&=\brak{\frac{2}{\pi}}^2\brak{\frac{\pi^2}{16} - 0}\\
    &=\frac{4\cdot{\pi}^2}{{\pi}^2\cdot16}\\
    &=\frac{1}{4}
    \end{align}