Variance of the random variable X is
\begin{align}
 V\brak{X} = E\brak{X^2}-\brak{E\brak{X}}^2   
\end{align}
\begin{lemma}
\begin{align}
    \int_{-\infty}^{\infty}xe^{-\frac{1}{2y}\brak{x-y}^2}\,dx = \sqrt{2\pi}y^\frac{3}{2}
\end{align}
\end{lemma}
\begin{proof}
\begin{align}
    &\int_{-\infty}^{\infty}xe^{-\frac{1}{2y}\brak{x-y}^2}\,dx\\
  =&\int_{-\infty}^{\infty}\brak{x-y}e^{-\frac{1}{2y}\brak{x-y}^2}\,dx+y\int_{-\infty}^{\infty}e^{-\frac{1}{2y}\brak{x-y}^2}\,dx\\
 =&0+\sqrt{2\pi}y^{\frac{3}{2}}\int_{-\infty}^{\infty}\frac{1}{\sqrt{y}\sqrt{2\pi}}e^{\frac{-1}{2\brak{\sqrt{y}}^2}\brak{x-y}^2}\,dx\\
 =&\sqrt{2\pi}y^\frac{3}{2}\lim_{x_0 \to -\infty}Q\brak{\frac{x_0 - y}{\sqrt{y}}}\\
  =&\sqrt{2\pi}y^\frac{3}{2} \label{twoD/2/eq:2}
\end{align}
\end{proof}
\begin{lemma}
\begin{align}
E\brak{X} = \frac{1}{2}
\end{align}
\end{lemma}
\begin{proof}
\begin{align}
 E\brak{X}=&\int_{0}^{1}\int_{-\infty}^{\infty}x f_{XY}\brak{x,y}\,dx\,dy\\
    =&\int_{0}^{1}\int_{-\infty}^{\infty}x\frac{1}{\sqrt{2\pi y}}e^{\frac{-1}{2y}\brak{x-y}^2}\,dx \,dy\\
     =&\int_{0}^{1}\frac{1}{\sqrt{2\pi y}}\brak{\int_{-\infty}^{\infty}xe^{-\frac{1}{2y}\brak{x-y}^2}\,dx}\,dy \label{twoD/2/eq:1}
\end{align}
From \eqref{twoD/2/eq:1} and \eqref{twoD/2/eq:2}, 
\begin{align}
E\brak{X}=&\int_{0}^{1}y\,dy\\
E\brak{X}=&\frac{1}{2} \label{twoD/2/eq:3}
\end{align}
\end{proof}
\begin{lemma}
\begin{align}
\int_{-\infty}^{\infty}x^2e^{-\frac{1}{2y}\brak{x-y}^2}\,dx=\sqrt{2\pi}y^\frac{3}{2}\brak{y+1}
\end{align}
\end{lemma} 
\begin{proof}
\begin{align}
&\int_{-\infty}^{\infty}x^2e^{-\frac{1}{2y}\brak{x-y}^2}\,dx\\
&=\brak{\sqrt{\frac{\pi}{2}}y^\frac{3}{2}\brak{y+1}\brak{1-2Q\brak{\frac{x-y}{\sqrt{y}}}} - ye^\frac{-\brak{x-y}^2}{2y}\brak{x+y}}]_{-\infty}^{\infty}\\
&=0-\sqrt{2\pi}y^\frac{3}{2}\brak{y+1}Q\brak{\frac{x-y}{\sqrt{y}}}]_{-\infty}^{\infty} - 0\\
&=\sqrt{2\pi}y^\frac{3}{2}\brak{y+1} \label{twoD/2/eq:5}
\end{align}
\end{proof}
\begin{lemma}
\begin{align}
E\brak{X^2} = \frac{5}{6}
\end{align}
\end{lemma}
\begin{proof}
\begin{align}
 E\brak{X^2}=&\int_{0}^{1}\int_{-\infty}^{\infty}x^2\,f_{XY}\brak{x, y}\,dx\,dy\\   
 =&\int_{0}^{1}\int_{-\infty}^{\infty}x^2\frac{1}{\sqrt{2\pi y}}e^{\frac{-1}{2y}\brak{x-y}^2}\,dx \,dy\\
 =&\int_{0}^{1}\frac{1}{\sqrt{2\pi y}}\brak{\int_{-\infty}^{\infty}x^2e^{-\frac{1}{2y}\brak{x-y}^2}\,dx}\,dy
 \label{twoD/2/eq:4}
\end{align}
From \eqref{twoD/2/eq:4} and \eqref{twoD/2/eq:5}, we get
\begin{align}
E\brak{X^2} = \int_{0}^{1}y\brak{y+1}dy\\
&=\brak{\frac{y^3}{3}+\frac{y^2}{2}}]_{0}^{1}\\
&=\frac{1}{3}+\frac{1}{2}=\frac{5}{6} \label{twoD/2/eq:6}
\end{align}
\end{proof}
From \eqref{twoD/2/eq:3} and \eqref{twoD/2/eq:6}, we get
\begin{align}
V\brak{X} = E\brak{X^2} - \brak{E\brak{X}}^2\\
     = \frac{5}{6} - \frac{1}{4}\\
     = \frac{7}{12}
\end{align}
Therefore, the answer is (C)$\frac{7}{12}$