\begin{enumerate}
    \item Given that $X_1$ is an exponential random variable. Let the P.D.F of $X_1$ be
    \begin{align}
    p_{X_1}(x_1)=
        \begin{cases}
        \lambda e^{-\lambda x_1} & x_1 \geq 0\\
        0 & x_1<0
        \end{cases}
    \end{align}
    C.D.F of $x_1$ is :
    \begin{align}
    \begin{split}
        F_{X_1}(x_1)&=\int_{-\infty}^{x_1} p_{X_1}(x_1) dx_1\\
        &=\int_{-\infty}^0 p_{X_1}(x_1) dx_1+\int_{0}^{x_1} p_{X_1}(x_1) dx_1\\
        &=\int_{-\infty}^0 0 \times dx_1+\int_{0}^ {x_1} \lambda e^{-\lambda x_1} dx_1\\
        &=1-e^{-\lambda x_1}\label{ec55:eq:0.0.2}
        \end{split}
    \end{align}
    \begin{align}
    \text{ As mean}=\lambda\\
     \text{ Given that mean}=1\\
     \text{so } \lambda=1 \label{ec55:eq:0.0.5}
    \end{align} 
     
    \item Given that $X_2$ is an gamma random variable.Let the P.D.F of $X_2$ be:
    \begin{align}
        p_{X_2}(x_2)=
        \begin{cases}
            \frac{a^b x_2^{b-1}e^{-ax_2}}{\Gamma(b)} & x_2\geq 0\\
            0 & x_2<0
        \end{cases}\label{ec55:eq:0.0.6}
    \end{align}
    \begin{align}
       \text{ Since mean}=\frac{b}{a}=2\label{ec55:eq:0.0.7}\\
         \text{Also,variance}=\frac{b}{a^2}=2\label{ec55:eq:0.0.8}
    \end{align}
  From \eqref{ec55:eq:0.0.7} and \eqref{ec55:eq:0.0.8}
  \begin{align}
      b=2,a=1\label{ec55:eq:0.0.9}
  \end{align}
  Since the total probability of $X_2$ is 1 \\
  so,\begin{align}
      \int_{-\infty}^\infty p_{X_2}(x_2) dx_2=1
      \end{align}
      \begin{align}
      \int_{-\infty} ^0 p_{X_2}(x_2)
     dx_2+\int_{0}^\infty p_{X_2}(x_2) dx_2&=1\\
      \int_{-\infty} ^0 0\times dx_2+\int_{0}^\infty \frac{a^b x_2^{b-1}e^{-ax_2}}{\Gamma(b)} dx_2&=1
      \end{align}
      \begin{align}
      \frac{a^b}{\Gamma(b)} \int_{0}^\infty x_2^{b-1}e^{-ax_2} dx_2&=1
      \end{align}
      \begin{align}
          \int_{0}^\infty x_2^{b-1}e^{-ax_2} dx_2&=\frac{\Gamma(b)}{a^b}\label{ec55:eq:0.0.14}
  \end{align}
  now substituting $a+\lambda$ for a in \eqref{ec55:eq:0.0.14} gives 
  \begin{align}
      \int_{0}^\infty x_2^{b-1}e^{-(a+\lambda)x_2} dx_2&=\frac{\Gamma(b)}{(a+\lambda)^b}\label{ec55:eq:0.0.15}
  \end{align}
  Now we have to find $P(X_1<X_2)$\\
  \item Given that $X_1$ and $X_2$ are independent random variables,so
  \begin{align}
     P(X_1<X_2|X_2)=F_{X_1}(X_2)=1-e^{-\lambda X_2}\label{ec55:eq:0.0.16}
  \end{align}
  Now,
\begin{align}
      P(X_1<X_2)&=\int_{0}^\infty F_{X_1}(X_2) \times p_{X_2}(x_2)dx_2
      \end{align}
      from \eqref{ec55:eq:0.0.6},\eqref{ec55:eq:0.0.16}
  \begin{align}
     P(X_1<X_2)=\int_{0}^\infty (1-e^{-\lambda X_2})\times \frac{a^b x_2^{b-1}e^{-ax_2}}{\Gamma(b)} dx_2
     \end{align}
     \begin{align}
     P(X_1<X_2)=\frac{a^b}{\Gamma(b)}\int_{0}^\infty x_2^{b-1}(e^{-ax_2}-e^{-(a+\lambda)x_2})dx_2
  \end{align}
      from \eqref{ec55:eq:0.0.14} and \eqref{ec55:eq:0.0.15}
      \begin{align}
     P(X_1<X_2)&=\frac{a^b}{\Gamma(b)}\brak{\frac{\Gamma(b)}{a^b}-\frac{\Gamma(b)}{(a+\lambda)^b}}
     \end{align}
 \begin{align}
      P(X_1<X_2)=1-\frac{a^b}{(a+\lambda)^b}
 \end{align}
 \begin{align}
     P(X_1<X_2)=1-\brak{\frac{a}{a+\lambda}}^b
 \end{align}
 from \eqref{ec55:eq:0.0.5} and \eqref{ec55:eq:0.0.9}
 \begin{align}
     P(X_1<X_2)&=1-\brak{\frac{1}{1+1}}^2\\
     P(X_1<X_2)&=1-\frac{1}{4}=\frac{3}{4}
 \end{align}
\end{enumerate}
