We know that,
\begin{equation}
    f_{Y|X=x}(y)=\frac{f(x,y)}{f_{X}(x)} \label{ec56:eq:2.0.1}
\end{equation}
Given that $f_{Y|X=x}(y)$ is uniform over the interval (x-1,x+1).
\begin{equation}
    \Rightarrow f_{Y|X=x}(y)=
    \begin{cases}
    \frac{1}{2} & y \in \brak{x-1,x+1}\\
    0 & \text{otherwise}
    \end{cases}\label{ec56:eq:2.0.2}
\end{equation}
Given $E(X)=1$
\begin{equation}
    \Rightarrow \int_{-\infty}^{\infty}x f_{X}(x)dx=1 \label{ec56:eq:2.0.3}
\end{equation}
Now consider $E(Y|X=x)$,
\begin{equation}
    E(Y|X=x)=\int_{-\infty}^{\infty}yf_{Y|X=x}(y)dy
\end{equation}
From \eqref{ec56:eq:2.0.2} it simplifies to,
\begin{multline}
    \Rightarrow E(Y|X=x)=\int_{-\infty}^{x-1}yf_{Y|X=x}(y)dy+\\ \int_{x-1}^{x+1}yf_{Y|X=x}(y)dy+\int_{x+1}^{\infty}yf_{Y|X=x}(y)dy
\end{multline}
\begin{align}
    \Rightarrow E(Y|X=x)&=\int_{x-1}^{x+1}y\brak{\frac{1}{2}}dy\\
    &=x
\end{align}
Now we can write ,\\
\begin{align}
    E(Y)&=\int_{-\infty}^{\infty}E(Y|X=x)f_{X}(x)dx\\
    &=\int_{-\infty}^{\infty}xf_{X}(x)dx\\
    &=E(X)
\end{align}
From \eqref{ec56:eq:2.0.3} we get 
\begin{equation}
    E(Y)=1.
\end{equation}