

Let the CDF of $f\brak{x}$ be denoted by $F_X\brak{x}$ \\
We know that,
\begin{align}
d\brak{F_X\brak{x}} = f\brak{x} \,dx \label{in2013-16Eq:1}
\end{align}
Therefore, applying definite integral on both sides from 0 to x in \eqref{in2013-16Eq:1}, we get,
\begin{align}
\int\limits_{0}^{x} d\brak{F_X\brak{x}} = \int\limits_{0}^{x} f\brak{x} \,dx = \int\limits_{0}^{x} e^{-x} \,dx \notag \\
F_X\brak{x} - F_X\brak{0} = e^{-0} - e^{-x} = 1 - e^{-x}   \label{in2013-16Eq:4}
\end{align}
We know that, there is no probability for the random variable X to satisfy $X \leq 0$,So, for $x = 0$ $F_X\brak{0}$ should be zero.So,
\begin{align}
F_X\brak{0} = 0 \label{in2013-16Eq:8}
\end{align}
Substituting \eqref{in2013-16Eq:8} in \eqref{in2013-16Eq:4}, we get
\begin{align}
F_X\brak{x} = 1 - e^{-x} \label{in2013-16Eq:12}
\end{align}
We know that,by definition 
\begin{align}
\pr{X > x} = 1-F_X\brak{x} \label{in2013-16Eq:13}
\end{align}
Substituting \eqref{in2013-16Eq:12} and x=1 in \eqref{in2013-16Eq:13}, we get
\begin{align}
\pr{X>1}=1-F_X\brak{1}=1-\brak{1-e^{-1}} \\
\pr{X>1}=e^{-1}
\end{align}
Therefore, \pr{X>1} = $\frac{1}{e}$